@prefix rdf: <http://www.w3.org/1999/02/22-rdf-syntax-ns#> .
@prefix owl: <http://www.w3.org/2002/07/owl#> .
@prefix xsd: <http://www.w3.org/2001/XMLSchema#> .
@prefix dcat: <http://www.w3.org/ns/dcat#> .
@prefix rdfs: <http://www.w3.org/2000/01/rdf-schema#> .
@prefix dctype: <http://purl.org/dc/dcmitype/> .
@prefix dct: <http://purl.org/dc/terms/> .

<http://www.w3.org/ns/dcat>
    dct:modified "2012-04-24"^^xsd:date ;
    a owl:Ontology ;
    rdfs:comment "DCAT is an RDF vocabulary designed to facilitate interoperability between data catalogs published on the Web." ;
    rdfs:label "The data catalog vocabulary" .

dcat:Catalog
    a rdfs:Class, owl:Class ;
    rdfs:comment "A  curated collection of metadata about datasets" ;
    rdfs:isDefinedBy <http://www.w3.org/ns/dcat> ;
    rdfs:label "Catalog" .

dcat:CatalogRecord
    a rdfs:Class, owl:Class ;
    rdfs:comment "A record in a data catalog, describing a single dataset" ;
    rdfs:isDefinedBy <http://www.w3.org/ns/dcat> ;
    rdfs:label "Catalog Record" .

dcat:Dataset
    a rdfs:Class, owl:Class ;
    rdfs:comment "A collection of data, published or curated by a single source, and available for access or download in one or more formats" ;
    rdfs:isDefinedBy <http://www.w3.org/ns/dcat> ;
    rdfs:label "Dataset" ;
    rdfs:subClassOf dctype:Dataset .

dcat:Distribution
    a rdfs:Class, owl:Class ;
    rdfs:comment "represents a specific available form of a dataset. Each dataset might be available in different forms, these forms might represent different formats of the dataset, different endpoints,... Examples of Distribution include a downloadable CSV file, an XLS file representing the dataset, an RSS feedâ€¦" ;
    rdfs:isDefinedBy <http://www.w3.org/ns/dcat> ;
    rdfs:label "Distribution" .

dcat:Download
    a rdfs:Class, owl:Class ;
    rdfs:comment "represents a downloadable distribution of a dataset" ;
    rdfs:isDefinedBy <http://www.w3.org/ns/dcat> ;
    rdfs:label "Download" ;
    rdfs:subClassOf dcat:Distribution .

dcat:Feed
    a rdfs:Class, owl:Class ;
    rdfs:comment "represents availability of a dataset as a feed" ;
    rdfs:isDefinedBy <http://www.w3.org/ns/dcat> ;
    rdfs:label "Feed" ;
    rdfs:subClassOf dcat:Distribution .

dcat:WebService
    a rdfs:Class, owl:Class ;
    rdfs:comment "represents a web service that enables access to the data of a dataset" ;
    rdfs:isDefinedBy <http://www.w3.org/ns/dcat> ;
    rdfs:label "Web Service" ;
    rdfs:subClassOf dcat:Distribution .

dcat:accessURL
    a rdf:Property ;
    rdfs:comment "points to the location of a distribution. This can be a direct download link, a link to an HTML page containing a link to the actual data, Feed, Web Service etc. the semantic is determined by its domain (Distribution, Feed, WebService, Download)" ;
    rdfs:isDefinedBy <http://www.w3.org/ns/dcat> ;
    rdfs:label "access URL" ;
    rdfs:range rdfs:Resource .

dcat:bytes
    a rdf:Property, owl:DatatypeProperty ;
    rdfs:comment "describe size of resource in bytes" ;
    rdfs:domain dcat:Distribution ;
    rdfs:isDefinedBy <http://www.w3.org/ns/dcat> ;
    rdfs:label "size in bytes" ;
    rdfs:range xsd:integer .

dcat:dataDictionary
    a rdf:Property ;
    rdfs:comment "links a dataset to a dictionary that helps interpreting the data" ;
    rdfs:domain dcat:Dataset ;
    rdfs:isDefinedBy <http://www.w3.org/ns/dcat> ;
    rdfs:label "data dictionary" .

dcat:dataQuality
    a rdf:Property ;
    rdfs:comment "describes the quality of data e.g. precision. This should not be used to describe the data collection characteristics, other more specialized statistical properties can be used instead." ;
    rdfs:domain dcat:Dataset ;
    rdfs:isDefinedBy <http://www.w3.org/ns/dcat> ;
    rdfs:label "data quality" .

dcat:dataset
    a rdf:Property ;
    rdfs:comment "a dataset that is part of the catalog" ;
    rdfs:domain dcat:Catalog ;
    rdfs:isDefinedBy <http://www.w3.org/ns/dcat> ;
    rdfs:label "dataset" ;
    rdfs:range dcat:Dataset .

dcat:distribution
    a rdf:Property ;
    rdfs:comment "connects a dataset to one of its available distributions" ;
    rdfs:domain dcat:Dataset ;
    rdfs:isDefinedBy <http://www.w3.org/ns/dcat> ;
    rdfs:label "distribution" ;
    rdfs:range dcat:Distribution .

dcat:granularity
    a rdf:Property ;
    rdfs:comment "describes the level of granularity of data in a dataset. The granularity can be in time, place etc" ;
    rdfs:domain dcat:Dataset ;
    rdfs:isDefinedBy <http://www.w3.org/ns/dcat> ;
    rdfs:label "granularity" .

dcat:keyword
    a rdf:Property ;
    rdfs:comment "a keyword or tag describing the datase" ;
    rdfs:isDefinedBy <http://www.w3.org/ns/dcat> ;
    rdfs:label "keyword" ;
    rdfs:range rdfs:Literal ;
    rdfs:subPropertyOf dct:subject .

dcat:record
    a rdf:Property ;
    rdfs:comment "links a catalog to its records" ;
    rdfs:domain dcat:Catalog ;
    rdfs:isDefinedBy <http://www.w3.org/ns/dcat> ;
    rdfs:label "record" ;
    rdfs:range dcat:CatalogRecord .

dcat:size
    a rdf:Property ;
    rdfs:comment "the size of a distribution" ;
    rdfs:domain dcat:Distribution ;
    rdfs:isDefinedBy <http://www.w3.org/ns/dcat> ;
    rdfs:label "size" ;
    rdfs:subPropertyOf dct:extent .

dcat:theme
    a rdf:Property ;
    rdfs:comment "the main category of the dataset. A dataset can have multiple themes" ;
    rdfs:isDefinedBy <http://www.w3.org/ns/dcat> ;
    rdfs:label "theme" ;
    rdfs:range <http://www.w3.org/2004/02/skos/core#Concept> ;
    rdfs:subPropertyOf dct:subject .

dcat:themeTaxonomy
    a rdf:Property ;
    rdfs:comment "the knowledge organization system (KOS) used to classify catalog's datasets" ;
    rdfs:domain dcat:Catalog ;
    rdfs:isDefinedBy <http://www.w3.org/ns/dcat> ;
    rdfs:label "themes" ;
    rdfs:range <http://www.w3.org/2004/02/skos/core#ConceptScheme> .

