@prefix rdf: <http://www.w3.org/1999/02/22-rdf-syntax-ns#> .
@prefix xsd: <http://www.w3.org/2001/XMLSchema#> .
@prefix rdfs: <http://www.w3.org/2000/01/rdf-schema#> .
@prefix owl: <http://www.w3.org/2002/07/owl#> .
@prefix wdrs: <http://www.w3.org/2007/05/powder-s#> .

<file:///Users/seebi/aksw.org/vocabularies/wdrs.rdf>
    a owl:Ontology ;
    rdfs:comment "This file specifies the set of classes and properties used in the RDF/OWL version of POWDER documents." ;
    rdfs:label "POWDER-S Vocabulary" ;
    owl:priorVersion <file:///Users/seebi/aksw.org/vocabularies/wdrs.rdf> ;
    owl:versionInfo "8 November 2010" .

<file:///Users/seebi/aksw.org/vocabularies/wdrs.rdf#Document>
    a rdfs:Class ;
    rdfs:comment "A POWDER document."@en ;
    rdfs:isDefinedBy <http://www.w3.org/TR/powder-dr/#structure> ;
    rdfs:label "POWDER document"@en ;
    rdfs:subClassOf owl:Ontology .

<file:///Users/seebi/aksw.org/vocabularies/wdrs.rdf#Processor>
    a rdfs:Class ;
    rdfs:comment "A software agent able to process POWDER documents."@en ;
    rdfs:isDefinedBy <http://www.w3.org/TR/powder-dr/#powderprocessor> ;
    rdfs:label "POWDER processor"@en ;
    rdfs:subClassOf <http://purl.org/dc/terms/Agent> .

<file:///Users/seebi/aksw.org/vocabularies/wdrs.rdf#authenticate>
    a rdf:Property ;
    rdfs:comment "A pointer to a document that describes how Description Resources created by a FOAF Agent or a DC Terms Agent may be authenticated"@en ;
    rdfs:isDefinedBy <http://www.w3.org/TR/powder-dr/#discover> ;
    rdfs:label "authenticate"@en .

<file:///Users/seebi/aksw.org/vocabularies/wdrs.rdf#certified>
    a rdf:Property ;
    rdfs:comment "A property that takes a Boolean value to declare whether the author of the data certifies the described resource."@en ;
    rdfs:isDefinedBy <http://www.w3.org/TR/powder-dr/#certification> ;
    rdfs:label "certified"@en ;
    rdfs:range xsd:boolean .

<file:///Users/seebi/aksw.org/vocabularies/wdrs.rdf#certifiedby>
    a rdf:Property, owl:AnnotationProperty ;
    rdfs:comment "A property that links a resource to a POWDER document that certifies it."@en ;
    rdfs:isDefinedBy <http://www.w3.org/TR/powder-dr/#certification> ;
    rdfs:label "certified by"@en .

<file:///Users/seebi/aksw.org/vocabularies/wdrs.rdf#data_error>
    a rdf:Property ;
    rdfs:comment "A property denoting a description of the specific error found in a given POWDER document."@en ;
    rdfs:domain <file:///Users/seebi/aksw.org/vocabularies/wdrs.rdf#Document> ;
    rdfs:isDefinedBy <http://www.w3.org/TR/powder-dr/#ppErrorhandling> ;
    rdfs:label "data error"@en .

<file:///Users/seebi/aksw.org/vocabularies/wdrs.rdf#describedby>
    a rdf:Property ;
    rdfs:comment "An RDF property to exactly match the describedby relationship type introduced in http://www.w3.org/TR/powder-dr/#assoc-linking and formally defined in appendix D of the same document, i.e. the relationship A 'describedby' B asserts that resource B provides a description of resource A. There are no constraints on the format or representation of either A or B, neither are there any further constraints on either resource."@en ;
    rdfs:isDefinedBy <http://www.w3.org/TR/powder-dr/#semlink> ;
    rdfs:label "described by"@en .

<file:///Users/seebi/aksw.org/vocabularies/wdrs.rdf#error_code>
    a rdf:Property ;
    rdfs:comment "A property denoting the code of any error encountered by the POWDER processor."@en ;
    rdfs:isDefinedBy <http://www.w3.org/TR/powder-dr/#ppErrorhandling> ;
    rdfs:label "error code"@en ;
    rdfs:range xsd:nonNegativeInteger .

<file:///Users/seebi/aksw.org/vocabularies/wdrs.rdf#hasIRI>
    a rdf:Property, owl:DatatypeProperty ;
    rdfs:comment "This property is meant to be used in OWL2 instead of wdrs:matchesregex. It denotes the string data range corresponding to a set of IRIs."@en ;
    rdfs:domain rdfs:Resource ;
    rdfs:isDefinedBy <http://www.w3.org/TR/powder-formal/#oxRegexSemantics> ;
    rdfs:label "has IRI"@en ;
    rdfs:range xsd:anyURI .

<file:///Users/seebi/aksw.org/vocabularies/wdrs.rdf#issuedby>
    a rdf:Property, owl:AnnotationProperty ;
    rdfs:comment "This property denotes the author of a POWDER document."@en ;
    rdfs:isDefinedBy <http://www.w3.org/TR/powder-dr/#line3> ;
    rdfs:label "issued by"@en .

<file:///Users/seebi/aksw.org/vocabularies/wdrs.rdf#logo>
    a rdf:Property, owl:AnnotationProperty ;
    rdfs:comment "Points to a graphic summary for the resources in a given class. Typically, it is a logo denoting conformance of a given (set of) resource(s) to a given set of criteria."@en ;
    rdfs:isDefinedBy <http://www.w3.org/TR/powder-dr/#line13> ;
    rdfs:label "logo"@en .

<file:///Users/seebi/aksw.org/vocabularies/wdrs.rdf#matchesregex>
    a rdf:Property, owl:DatatypeProperty ;
    rdfs:comment "This is the key 'include' property for IRI set definitions in POWDER-S. It is necessary to take account of the POWDER Semantic Extension to process this fully. The value is a regular expression that is matched against an IRI."@en ;
    rdfs:domain rdfs:Resource ;
    rdfs:isDefinedBy <http://www.w3.org/TR/powder-formal/#regexSemantics> ;
    rdfs:label "matches regular expression"@en ;
    rdfs:range xsd:string ;
    rdfs:seeAlso <http://www.w3.org/TR/xpath-functions/#regex-syntax> .

<file:///Users/seebi/aksw.org/vocabularies/wdrs.rdf#notknownto>
    a rdf:Property ;
    rdfs:comment "Property used in results returned from a POWDER Processor that has no data about the candidate resource. The value is the IRI of the processor."@en ;
    rdfs:isDefinedBy <http://www.w3.org/TR/powder-dr/#powderprocessor> ;
    rdfs:label "not known to"@en ;
    rdfs:range <file:///Users/seebi/aksw.org/vocabularies/wdrs.rdf#Processor> .

<file:///Users/seebi/aksw.org/vocabularies/wdrs.rdf#notmatchesregex>
    a rdf:Property, owl:DatatypeProperty ;
    rdfs:comment "This is the key 'exclude' property for IRI set definitions in POWDER-S. It is necessary to take account of the POWDER Semantic Extension to process this fully. The value is a regular expression that is matched against an IRI."@en ;
    rdfs:domain rdfs:Resource ;
    rdfs:isDefinedBy <http://www.w3.org/TR/powder-formal/#regexSemantics> ;
    rdfs:label "matches regular expression"@en ;
    rdfs:range xsd:string ;
    rdfs:seeAlso <http://www.w3.org/TR/xpath-functions/#regex-syntax> .

<file:///Users/seebi/aksw.org/vocabularies/wdrs.rdf#proc_error>
    a rdf:Property ;
    rdfs:comment "A property denoting a description of the specific software error."@en ;
    rdfs:domain <file:///Users/seebi/aksw.org/vocabularies/wdrs.rdf#Processor> ;
    rdfs:isDefinedBy <http://www.w3.org/TR/powder-dr/#ppErrorhandling> ;
    rdfs:label "processing error"@en .

<file:///Users/seebi/aksw.org/vocabularies/wdrs.rdf#sha1sum>
    a rdf:Property ;
    rdfs:comment "Links to a Base64-encoded binary SHA-1 hash of the described resource. May be used by POWDER Processors when assessing trustworthiness of a DR."@en ;
    rdfs:isDefinedBy <http://www.w3.org/TR/powder-dr/#certification> ;
    rdfs:label "SHA-1 sum"@en ;
    rdfs:range xsd:base64Binary .

<file:///Users/seebi/aksw.org/vocabularies/wdrs.rdf#supportedby>
    a rdf:Property, owl:AnnotationProperty ;
    rdfs:comment "A property that links a POWDER document to some other data source that supports the descriptions provided."@en ;
    rdfs:isDefinedBy <http://www.w3.org/TR/powder-dr/#supportedBy> ;
    rdfs:label "supported by"@en .

<file:///Users/seebi/aksw.org/vocabularies/wdrs.rdf#tag>
    a rdf:Property, owl:DatatypeProperty ;
    rdfs:comment "Property linking to a free-text tag which may include spaces."@en ;
    rdfs:isDefinedBy <http://www.w3.org/TR/powder-dr/#tags> ;
    rdfs:label "tag"@en ;
    rdfs:range xsd:token .

<file:///Users/seebi/aksw.org/vocabularies/wdrs.rdf#text>
    a rdf:Property, owl:AnnotationProperty ;
    rdfs:comment "This property provides a summary of the descriptorset that it annotates, suitable for display to end users."@en ;
    rdfs:isDefinedBy <http://www.w3.org/TR/powder-dr/#line13> ;
    rdfs:label "text that may be displayed"@en .

<file:///Users/seebi/aksw.org/vocabularies/wdrs.rdf#validfrom>
    a rdf:Property, owl:AnnotationProperty ;
    rdfs:comment "Provides a timestamp that a POWDER Processor may use when assessing trustworthiness of a POWDER document. Informally, a POWDER Processor should normally ignore data in the document before the given date."@en ;
    rdfs:isDefinedBy <http://www.w3.org/TR/powder-dr/#certification> ;
    rdfs:label "valid from"@en .

<file:///Users/seebi/aksw.org/vocabularies/wdrs.rdf#validuntil>
    a rdf:Property, owl:AnnotationProperty ;
    rdfs:comment "Provides a timestamp that a POWDER Processor may use when assessing trustworthiness of a POWDER document. Informally, a POWDER Processor should normally ignore data in the document after the given date."@en ;
    rdfs:isDefinedBy <http://www.w3.org/TR/powder-dr/#certification> ;
    rdfs:label "valid until"@en .

